Define the future and the le relations on the memory

src/lang/Memory.v
@@ -66,14 +66,20 @@ Module Cell.
       forall to from msg
         (MESSAGE: messages to = Some (from, msg)),
         Time.lt from to;
+    DISJOINT:
+      forall to1 to2 from1 from2 msg1 msg2
+        (TO: to1 <> to2)
+        (MESSAGE1: messages to1 = Some (from1, msg1))
+        (MESSAGE2: messages to2 = Some (from2, msg2)),
+        Interval.disjoint (from1, to1) (from2, to2);
+    DOMAIN:
+      exists tos,
+      forall to from msg (MSG: messages to = Some (from, msg)),
+        List.In to tos;
   }.
 
-  Definition wf (cell:t): Prop :=
-    forall to1 to2 from1 from2 msg1 msg2
-      (TO: to1 <> to2)
-      (MESSAGE1: cell.(messages) to1 = Some (from1, msg1))
-      (MESSAGE2: cell.(messages) to2 = Some (from2, msg2)),
-      Interval.disjoint (from1, to1) (from2, to2).
+  Definition get (to:Time.t) (cell:t): option Message.t :=
+    option_map snd (cell.(messages) to).
 
   Lemma extensionality lhs rhs
         (MESSAGES: forall x, lhs.(messages) x = rhs.(messages) x):
@@ -81,40 +87,13 @@ Module Cell.
   Proof.
     destruct lhs, rhs.
     cut (messages0 = messages1).
-    { i. subst. f_equal. apply proof_irrelevance. }
+    { i. subst. f_equal; apply proof_irrelevance. }
     extensionality to. auto.
   Qed.
 
   Definition le (lhs rhs:t): Prop :=
     forall to from msg (MSG: lhs.(messages) to = Some (from, msg)),
       rhs.(messages) to = Some (from, msg).
-
-  Program Definition init: t :=
-    mk
-      (TimeFun.add Time.elt (Some (Time.decr Time.elt, Message.mk 0 Snapshot.init)) (TimeFun.init None))
-      _.
-  Next Obligation.
-    unfold TimeFun.add in *.
-    match goal with
-    | [H: context[if ?c then _ else _] |- _] => destruct c
-    end;
-      inv MESSAGE.
-    apply Time.decr_spec.
-  Qed.
-
-  Lemma init_wf: wf init.
-  Proof.
-    unfold wf, init. i. simpl in *.
-    unfold TimeFun.add in *.
-    repeat
-      match goal with
-      | [H: context[if ?c then _ else _] |- _] => destruct c
-      | [H: Some _ = Some _ |- _] => inv H
-      end;
-      try inv MESSAGE1;
-      try inv MESSAGE2.
-    congruence.
-  Qed.
 
   Inductive own (cell:t) (ts:Time.t): Prop :=
   | own_intro
@@ -125,13 +104,6 @@ Module Cell.
 
   Definition disjoint (lhs rhs:t): Prop :=
     forall ts (LHS: own lhs ts) (RHS: own rhs ts), False.
-
-  Lemma disjoint_comm lhs rhs
-        (DISJ: disjoint lhs rhs):
-    disjoint rhs lhs.
-  Proof.
-    ii. eapply DISJ; eauto.
-  Qed.
 
   Lemma disjoint_messages
         to lhs rhs lx rx
@@ -146,150 +118,99 @@ Module Cell.
     - apply Interval.mem_ub. eapply VOLUME. eauto.
   Qed.
 
-  Program Definition join (lhs rhs:t): t :=
-    mk
-      (fun x =>
-         match lhs.(messages) x, rhs.(messages) x with
-         | Some _, Some _ => Some (Time.decr x, Message.elt)
-         | Some lhs, None => Some lhs
-         | None, Some rhs => Some rhs
-         | None, None => None
-         end)
-      _.
-  Next Obligation.
-    destruct (messages lhs to) as [[]|] eqn:LHS,
-             (messages rhs to) as [[]|] eqn:RHS; try inv MESSAGE.
-    - apply Time.decr_spec.
-    - exploit (lhs.(VOLUME)); eauto.
-    - exploit (rhs.(VOLUME)); eauto.
-  Qed.
-
-  Lemma join_wf
-        lhs rhs
-        (DISJ: disjoint lhs rhs)
-        (LHS: wf lhs)
-        (RHS: wf rhs):
-    wf (join lhs rhs).
-  Proof.
-    ii. simpl in *.
-    destruct (messages lhs to1) as [[]|] eqn:LHS1,
-             (messages rhs to1) as [[]|] eqn:RHS1;
-      inv MESSAGE1;
-    destruct (messages lhs to2) as [[]|] eqn:LHS2,
-             (messages rhs to2) as [[]|] eqn:RHS2;
-      inv MESSAGE2;
-      try (eapply (disjoint_messages to1); eauto; fail);
-      try (eapply (disjoint_messages to2); eauto; fail).
-    - eapply LHS; eauto.
-    - eapply DISJ; econs; eauto.
-    - eapply DISJ; econs; eauto.
-    - eapply RHS; eauto.
-  Qed.
-
-  Lemma join_assoc x y z:
-    join (join x y) z = join x (join y z).
-  Proof.
-    apply extensionality. simpl. i.
-    destruct (messages x x0), (messages y x0), (messages z x0); auto.
-  Qed.
-
-  Lemma join_le
-        lhs rhs
+  Lemma disjoint_comm lhs rhs
         (DISJ: disjoint lhs rhs):
-    le lhs (join lhs rhs).
+    disjoint rhs lhs.
   Proof.
-    unfold join. ii. simpl in *.
-    destruct (messages lhs to) as [[]|] eqn:LHS,
-             (messages rhs to) as [[]|] eqn:RHS;
-      try congruence.
-    exfalso. eapply disjoint_messages; eauto.
+    ii. eapply DISJ; eauto.
   Qed.
 
-  Lemma join_spec
-        lhs rhs b
-        (DISJ: disjoint lhs rhs)
-        (LHS: le lhs b)
-        (RHS: le rhs b):
-    le (join lhs rhs) b.
-  Proof.
-    unfold join. ii. simpl in *.
-    destruct (messages lhs to) as [[]|] eqn:LHS1,
-             (messages rhs to) as [[]|] eqn:RHS1;
-      inv MSG;
-      try congruence.
-    - exfalso. eapply disjoint_messages; eauto.
-    - apply LHS. auto.
-    - apply RHS. auto.
-  Qed.
-
-  Lemma join_comm lhs rhs:
-    join lhs rhs = join rhs lhs.
-  Proof.
-    apply extensionality. simpl. i.
-    destruct (messages lhs x), (messages rhs x); auto.
-  Qed.
-
-  Program Definition sub (lhs rhs:t): t :=
+  Program Definition init: t :=
     mk
-      (fun x =>
-         match lhs.(messages) x, rhs.(messages) x with
-         | _, Some _
-         | None, _ => None
-         | Some lhs, None => Some lhs
-         end)
-      _.
+      (TimeFun.add Time.elt (Some (Time.decr Time.elt, Message.mk 0 Snapshot.init)) (TimeFun.init None))
+      _ _ _.
   Next Obligation.
-    destruct (messages lhs to) eqn:LHS, (messages rhs to) eqn:RHS; inv MESSAGE.
+    unfold TimeFun.add in *.
+    match goal with
+    | [H: context[if ?c then _ else _] |- _] => destruct c
+    end;
+      inv MESSAGE.
+    apply Time.decr_spec.
+  Qed.
+  Next Obligation.
+    unfold TimeFun.add in *.
+    repeat match goal with
+           | [H: context[if ?c then _ else _] |- _] => destruct c
+           end;
+      subst; inv MESSAGE1; inv MESSAGE2.
+    congruence.
+  Qed.
+  Next Obligation.
+    exists [Time.elt]. i.
+    unfold TimeFun.add in *.
+    match goal with
+    | [H: context[if ?c then _ else _] |- _] => destruct c
+    end;
+      subst; inv MSG.
+    econs. auto.
+  Qed.
+
+  Inductive declare (from to:Time.t) (msg:Message.t) (cell1 cell2:t): Prop :=
+  | declare_add
+      (MESSAGES1: cell1.(messages) to = None)
+      (MESSAGES2: cell2.(messages) = TimeFun.add to (Some (from, msg)) cell1.(messages))
+  | declare_split
+      msg' middle
+      (MESSAGES1: cell1.(messages) to = Some (from, msg'))
+      (MESSAGES2: cell2.(messages) =
+                  TimeFun.add middle (Some (from, msg))
+                              (TimeFun.add to (Some (middle, msg)) cell1.(messages)))
+  .
+
+  Definition future: forall (lhs rhs:t), Prop :=
+    rtc (fun c1 c2 => exists from to msg, declare from to msg c1 c2).
+
+  Lemma declare_future
+        from to msg cell1 cell2
+        (DECLARE: declare from to msg cell1 cell2):
+    future cell1 cell2.
+  Proof.
+    econs 2; [|econs 1].
+    eexists _, _, _. eauto.
+  Qed.
+
+  Program Definition remove (to:Time.t) (cell:t): t :=
+    mk (TimeFun.add to None cell.(messages)) _ _ _.
+  Next Obligation.
+    unfold TimeFun.add in *.    match goal with
+    | [H: context[if ?c then _ else _] |- _] => destruct c
+    end; inv MESSAGE.
     eapply VOLUME; eauto.
   Qed.
-
-  Lemma sub_wf
-        lhs rhs
-        (LHS: wf lhs)
-        (RHS: wf rhs):
-    wf (sub lhs rhs).
-  Proof.
-    ii. simpl in *.
-    destruct (messages lhs to1) as [[]|] eqn:LHS1,
-             (messages rhs to1) as [[]|] eqn:RHS1;
-      inv MESSAGE1;
-    destruct (messages lhs to2) as [[]|] eqn:LHS2,
-             (messages rhs to2) as [[]|] eqn:RHS2;
-      inv MESSAGE2;
-      try (eapply (disjoint_messages to1); eauto; fail);
-      try (eapply (disjoint_messages to2); eauto; fail).
-    eapply LHS; eauto.
+  Next Obligation.
+    unfold TimeFun.add in *.    repeat match goal with
+           | [H: context[if ?c then _ else _] |- _] => destruct c
+           end;
+      inv MESSAGE1; inv MESSAGE2.
+    eapply DISJOINT; eauto.
   Qed.
-
-  Lemma sub_le lhs rhs:
-    le (sub lhs rhs) lhs.
-  Proof.
-    unfold sub. ii. simpl in *.
-    destruct (messages lhs to) as [[]|] eqn:LHS,
-             (messages rhs to) as [[]|] eqn:RHS;
-      congruence.
-  Qed.
-
-  Lemma sub_spec lhs rhs
-        (DISJ: disjoint lhs rhs):
-    sub (join lhs rhs) rhs = lhs.
-  Proof.
-    apply extensionality. simpl. i.
-    destruct (messages lhs x) as [[]|] eqn:LHS,
-             (messages rhs x) as [[]|] eqn:RHS;
-      try congruence.
-    exfalso. eapply disjoint_messages; eauto.
+  Next Obligation.
+    generalize (DOMAIN cell). i. des.
+    exists tos. i.
+    unfold TimeFun.add in *.    match goal with
+    | [H: context[if ?c then _ else _] |- _] => destruct c
+    end; inv MSG.
+    eapply H; eauto.
   Qed.
 End Cell.
 
 Module Memory.
   Definition t := Loc.t -> Cell.t.
-  Definition wf (mem:t): Prop := forall loc, Cell.wf (mem loc).
-  Definition le (lhs rhs:t): Prop := forall loc, Cell.le (lhs loc) (rhs loc).
 
-  Definition init: t := LocFun.init Cell.init.
-  Lemma init_wf: wf init.
-  Proof. intro loc. apply Cell.init_wf. Qed.
+  Definition get (loc:Loc.t) (to:Time.t) (mem:t): option Message.t :=
+    Cell.get to (mem loc).
+
+  Definition le (lhs rhs:t): Prop := forall loc, Cell.le (lhs loc) (rhs loc).
 
   Definition disjoint (lhs rhs:t): Prop :=
     forall loc, Cell.disjoint (lhs loc) (rhs loc).
@@ -302,134 +223,30 @@ Module Memory.
     apply Cell.disjoint_comm. auto.
   Qed.
 
-  Definition join (lhs rhs:t): t :=
-    fun loc => Cell.join (lhs loc) (rhs loc).
+  Definition init: t := LocFun.init Cell.init.
 
-  Lemma join_wf
-        lhs rhs
-        (DISJ: disjoint lhs rhs)
-        (LHS: wf lhs)
-        (RHS: wf rhs):
-    wf (join lhs rhs).
-  Proof. intro loc. apply Cell.join_wf; auto. Qed.
-
-  Lemma join_assoc x y z:
-    join (join x y) z = join x (join y z).
-  Proof. extensionality loc. apply Cell.join_assoc. Qed.
-
-  Lemma join_le
-        lhs rhs
-        (DISJ: disjoint lhs rhs):
-    le lhs (join lhs rhs).
-  Proof. intro loc. apply Cell.join_le; auto. Qed.
-
-  Lemma join_spec
-        lhs rhs b
-        (DISJ: disjoint lhs rhs)
-        (LHS: le lhs b)
-        (RHS: le rhs b):
-    le (join lhs rhs) b.
-  Proof. intro loc. apply Cell.join_spec; auto. Qed.
-
-  Lemma join_comm lhs rhs:
-    join lhs rhs = join rhs lhs.
-  Proof. extensionality loc. apply Cell.join_comm. Qed.
-
-  Definition sub (lhs rhs:t): t :=
-    fun loc => Cell.sub (lhs loc) (rhs loc).
-
-  Lemma sub_wf
-        lhs rhs
-        (LHS: wf lhs)
-        (RHS: wf rhs):
-    wf (sub lhs rhs).
-  Proof. intro loc. apply Cell.sub_wf; auto. Qed.
-
-  Lemma sub_le lhs rhs:
-    le (sub lhs rhs) lhs.
-  Proof. intro loc. apply Cell.sub_le. Qed.
-
-  Lemma sub_spec lhs rhs
-        (DISJ: disjoint lhs rhs):
-    sub (join lhs rhs) rhs = lhs.
-  Proof. extensionality loc. apply Cell.sub_spec. auto. Qed.
-End Memory.
-
-
-Module Memory.
-  Structure t := mk {
-    messages: MessageSet.t;
-    used: IntervalSets.t;
-  }.
-
-  Definition init: t := mk MessageSet.empty IntervalSets.bot.
-
-  Inductive step (thl1:ThreadLocal.t) (mem1:t): forall (e:option MemEvent.t) (thl2:ThreadLocal.t), Prop :=
-  | step_read
-      loc val ts released ord tc2
-      (READ: Commit.read thl1.(ThreadLocal.tc) loc ts released ord tc2)
-      (DECLARE: ~ IntervalSets.mem loc ts thl1.(ThreadLocal.declares))
-      (MESSAGE: MessageSet.get loc ts mem1.(messages) = Some (Message.mk val released)):
-      step thl1 mem1
-           (Some (MemEvent.read loc val ord))
-           (ThreadLocal.mk tc2 thl1.(ThreadLocal.declares))
-  | step_write
-      loc val ts0 ts released ord tc2 declares2
-      (WRITE: Commit.write thl1.(ThreadLocal.tc) loc ts released ord tc2)
-      (DECLARE: IntervalSets.remove loc ts0 ts thl1.(ThreadLocal.declares) = Some declares2)
-      (MESSAGE: MessageSet.get loc ts mem1.(messages) = Some (Message.mk val released)):
-      step thl1 mem1
-           (Some (MemEvent.write loc val ord))
-           (ThreadLocal.mk tc2 declares2)
-  | step_update
-      loc valr tsr releasedr valw tsw releasedw ord tc2 tc3 declares3
-      (READ: Commit.read thl1.(ThreadLocal.tc) loc tsr releasedr ord tc2)
-      (WRITE: Commit.write tc2 loc tsw releasedw ord tc3)
-      (RELEASE: Snapshot.le releasedr releasedw)
-      (DECLARE: IntervalSets.remove loc tsr tsw thl1.(ThreadLocal.declares) = Some declares3)
-      (MESSAGE1: MessageSet.get loc tsr mem1.(messages) = Some (Message.mk valr releasedr))
-      (MESSAGE2: MessageSet.get loc tsw mem1.(messages) = Some (Message.mk valw releasedw)):
-      step thl1 mem1
-           (Some (MemEvent.update loc valr valw ord))
-           (ThreadLocal.mk tc3 declares3)
-  | step_fence
-      ord tc2
-      (FENCE: Commit.fence thl1.(ThreadLocal.tc) ord tc2):
-      step thl1 mem1
-           (Some (MemEvent.fence ord))
-           (ThreadLocal.mk tc2 thl1.(ThreadLocal.declares))
-  | step_None
-      tc2
-      (COMMIT: Commit.le thl1.(ThreadLocal.tc) tc2):
-      step thl1 mem1
-           None
-           (ThreadLocal.mk tc2 thl1.(ThreadLocal.declares))
-  .
-
-  Inductive declare (thl1:ThreadLocal.t) (mem1:t): forall (thl2:ThreadLocal.t) (mem2:t), Prop :=
+  Inductive declare (loc:Loc.t) (from to:Time.t) (msg:Message.t) (mem1:t): forall (mem2:t), Prop :=
   | declare_intro
-      loc ts val released ts0 declares2 used2
-      (TS: Time.lt ts0 ts)
-      (LOCAL: ThreadLocal.declare loc ts0 ts thl1.(ThreadLocal.declares) mem1.(used) declares2 used2)
-      (GET: MessageSet.get loc ts mem1.(messages) = None):
-      declare thl1 mem1
-              (ThreadLocal.mk thl1.(ThreadLocal.tc) declares2)
-              (mk (MessageSet.set loc ts (Message.mk val released) mem1.(messages))
-                  used2)
+      cell2
+      (ALLOC: Cell.declare from to msg (mem1 loc) cell2):
+      declare loc from to msg mem1 (LocFun.add loc cell2 mem1)
   .
 
-  (* TODO: messages are in rhs.(used)? *)
-  Inductive future (declares:IntervalSets.t) (lhs rhs:t): Prop :=
-  | future_intro
-      (MESSAGE: forall loc ts, Message.future (MessageSet.get loc ts lhs.(messages)) (MessageSet.get loc ts rhs.(messages)))
-      (DECLARE:
-         forall loc ts (DECLARE: IntervalSets.mem loc ts declares),
-           MessageSet.get loc ts lhs.(messages) = MessageSet.get loc ts rhs.(messages))
-      (PERM: IntervalSets.le lhs.(used) rhs.(used))
-  .
+  Definition future: forall (lhs rhs:t), Prop :=
+    rtc (fun c1 c2 => exists loc from to msg, declare loc from to msg c1 c2).
+
+  Lemma declare_future
+        loc from to msg mem1 mem2
+        (DECLARE: declare loc from to msg mem1 mem2):
+    future mem1 mem2.
+  Proof.
+    econs 2; [|econs 1].
+    eexists _, _, _. eauto.
+  Qed.
+
+  Definition remove (loc:Loc.t) (to:Time.t) (mem:t): t :=
+    LocFun.add loc (Cell.remove to (mem loc)) mem.
 End Memory.
-
-
 
 
 Module Commit.
@@ -452,7 +269,7 @@ Module Commit.
             (tc1:t) (loc:Loc.t) (ts:Time.t) (released:Snapshot.t) (ord:Ordering.t)
             (tc2:t): Prop :=
   | read_intro
-      (FUTURE: le tc1 tc2)
+      (MONOTONE: le tc1 tc2)
       (READABLE: Snapshot.readable tc1.(current) loc ts)
       (READ: Time.le ts (Times.get loc tc2.(current).(Snapshot.reads)))
       (ACQUIRE: forall (ORDERING: Ordering.le Ordering.acquire ord),
@@ -464,7 +281,7 @@ Module Commit.
             (tc1:t) (loc:Loc.t) (ts:Time.t) (released:Snapshot.t) (ord:Ordering.t)
             (tc2:t): Prop :=
   | write_intro
-      (FUTURE: le tc1 tc2)
+      (MONOTONE: le tc1 tc2)
       (WRITABLE: Snapshot.writable tc1.(current) loc ts)
       (WRITE: Time.le ts (Times.get loc tc2.(current).(Snapshot.writes)))
       (RELEASE: forall (ORDERING: Ordering.le Ordering.release ord),
@@ -476,7 +293,7 @@ Module Commit.
             (tc1:t) (ord:Ordering.t)
             (tc2:t): Prop :=
   | fence_intro
-      (FUTURE: le tc1 tc2)
+      (MONOTONE: le tc1 tc2)
       (ACQUIRE: forall (ORDERING: Ordering.le Ordering.acquire ord),
           Snapshot.le tc2.(acquirable) tc2.(current))
       (RELEASE: forall (ORDERING: Ordering.le Ordering.release ord) loc,
@@ -486,27 +303,57 @@ End Commit.
 
 Module ThreadLocal.
   Structure t := mk {
-    tc: Commit.t;
-    declares: IntervalSets.t;
+    commit: Commit.t;
+    local: Memory.t;
   }.
 
-  Definition init := mk Commit.init IntervalSets.bot.
+  Definition init := mk Commit.init Memory.init.
 
-  Inductive declare
-            (loc:Loc.t) (ts0 ts:Time.t)
-            (declares1:IntervalSets.t) (used1:IntervalSets.t):
-    forall (declares2:IntervalSets.t) (used2:IntervalSets.t), Prop :=
-  | declare_alloc
-      (DISJOINT: IntervalSets.disjoint loc ts0 ts used1):
-      declare loc ts0 ts declares1 used1
-              (IntervalSets.add loc ts0 ts declares1)
-              (IntervalSets.add loc ts0 ts used1)
-  | declare_split
-      ts1 declares2
-      (TIME: Time.lt ts ts1)
-      (DECLARE: IntervalSets.remove loc ts0 ts1 declares1 = Some declares2):
-      declare loc ts0 ts declares1 used1
-              (IntervalSets.add loc ts0 ts (IntervalSets.add loc ts ts1 declares2))
-              used1
+  Inductive step (thl1:t) (mem1:Memory.t): forall (e:option MemEvent.t) (thl2:t), Prop :=
+  | step_read
+      loc val ts released ord commit2
+      (READ: Commit.read thl1.(commit) loc ts released ord commit2)
+      (MESSAGE: Memory.get loc ts mem1 = Some (Message.mk val released))
+      (LOCAL: Memory.get loc ts thl1.(local) = None):
+      step thl1 mem1
+           (Some (MemEvent.read loc val ord))
+           (mk commit2 thl1.(local))
+  | step_write
+      loc val ts released ord commit2
+      (WRITE: Commit.write thl1.(commit) loc ts released ord commit2)
+      (MESSAGE: Memory.get loc ts thl1.(local) = Some (Message.mk val released)):
+      step thl1 mem1
+           (Some (MemEvent.write loc val ord))
+           (mk commit2 (Memory.remove loc ts thl1.(local)))
+  | step_update
+      loc valr tsr releasedr valw tsw releasedw ord commit2 commit3
+      (READ: Commit.read thl1.(commit) loc tsr releasedr ord commit2)
+      (WRITE: Commit.write commit2 loc tsw releasedw ord commit3)
+      (RELEASE: Snapshot.le releasedr releasedw)
+      (MESSAGE1: Memory.get loc tsr mem1 = Some (Message.mk valr releasedr))
+      (MESSAGE2: Memory.get loc tsw thl1.(local) = Some (Message.mk valw releasedw)):
+      step thl1 mem1
+           (Some (MemEvent.update loc valr valw ord))
+           (mk commit3 (Memory.remove loc tsw thl1.(local)))
+  | step_fence
+      ord commit2
+      (FENCE: Commit.fence thl1.(commit) ord commit2):
+      step thl1 mem1
+           (Some (MemEvent.fence ord))
+           (mk commit2 thl1.(local))
+  | step_None
+      commit2
+      (COMMIT: Commit.le thl1.(commit) commit2):
+      step thl1 mem1
+           None
+           (mk commit2 thl1.(local))
+  .
+
+  Inductive declare (thl1:t) (mem1:Memory.t) (thl2:t) (mem2:Memory.t): Prop :=
+  | declare_intro
+      loc from to msg
+      (COMMIT: Commit.le thl1.(commit) thl2.(commit))
+      (LOCAL: Memory.declare loc from to msg thl1.(local) thl2.(local))
+      (MEMORY: Memory.declare loc from to msg mem1 mem2)
   .
 End ThreadLocal.
